src/m_in/ssfact.lean
@@ -19,7 +19,26 @@ instance empty_subset_ground : fact (∅ ⊆ E) := ⟨empty_subset _⟩
 
 instance ground_subset_ground : fact (E ⊆ E) := ⟨subset.rfl⟩
 
-@[simp] lemma set.subset_ground (X : set α) [fact (X ⊆ E)] : X ⊆ E := fact.elim ‹_›
+@[simp] lemma set.subset_ground (X E : set α) [fact (X ⊆ E)] : X ⊆ E := fact.elim ‹_›
+
+@[simp] lemma set.inter_ground (X E : set α) [fact (X ⊆ E)] : X ∩ E = X :=
+inter_eq_self_of_subset_left (X.subset_ground E)
+
+@[simp] lemma set.ground_inter (X E : set α) [fact (X ⊆ E)] : E ∩ X = X :=
+inter_eq_self_of_subset_right (X.subset_ground E)
+
+lemma rcompl_rcompl [fact (X ⊆ E)] : (E \ (E \ X)) = X := by simp 
+
+lemma rcompl_subset_rcompl (E : set α) [fact (X ⊆ E)] [fact (Y ⊆ E)] : (E \ X) ⊆ (E \ Y) ↔ Y ⊆ X :=
+begin
+  rw [←compl_subset_compl, diff_eq, compl_inter, diff_eq, compl_inter, compl_compl, compl_compl, 
+    union_subset_iff, and_iff_right (subset_union_left _ _)], 
+  refine ⟨λ h, _, λ h, h.trans (subset_union_right _ _)⟩,
+  rw [←Y.ground_inter E], 
+  refine (inter_subset_inter_right _ h).trans _, 
+  rw [inter_distrib_left, inter_compl_self, empty_union], 
+  exact inter_subset_right _ _, 
+end   
 
 -- lemma foo {E X : set α} {P : set α → Prop} (hP : ∀ Y, P Y → Y ⊆ E) : 
 --   X ∈ maximals (⊆) {Y | P Y} ↔ E \ X ∈ maximals (⊆) {Y | Y ⊆ E ∧ P (E \ Y)}  
